theories/generic/utp_subst.thy
@@ -16,10 +16,13 @@ begin
 subsection {* Variable Substitutions *}
 
 text {* Substitutions are total bijections and have to respect typing. *}
+definition VAR_SUBST_ON :: "'TYPE VAR set \<Rightarrow> (('TYPE VAR \<Rightarrow> 'TYPE VAR) set)" where
+"VAR_SUBST_ON a = {ss . bij_split ss a a \<and> (\<forall> v \<in> a . type (ss v) = type v)}"
 
-definition VAR_SUBST :: "('TYPE VAR \<Rightarrow> 'TYPE VAR) set" where
-"VAR_SUBST = {ss . bij ss \<and> (\<forall> v . type (ss v) = type v)}"
+abbreviation VAR_SUBST :: "('TYPE VAR \<Rightarrow> 'TYPE VAR) set" where
+"VAR_SUBST \<equiv> VAR_SUBST_ON UNIV"
 
+text {* mappings is the set of variables which are changed by the substitution *}
 definition mappings :: "('a \<Rightarrow> 'a) \<Rightarrow> 'a set" where
 "mappings f = {v. f v \<noteq> v} \<union> {v. (inv f) v \<noteq> v}"
 
@@ -32,7 +35,7 @@ lemma disj_mapping_comm: "\<lbrakk> inj f; inj g; mappings f \<inter> mappings g
   apply(smt inv_f_f)
 done
 
-lemma disj_mapping_image: "\<lbrakk> mappings f \<inter> a = {} \<rbrakk> \<Longrightarrow> f ` a = a"
+lemma disj_mapping_image[alphabet]: "\<lbrakk> mappings f \<inter> a = {} \<rbrakk> \<Longrightarrow> f ` a = a"
   apply(auto simp add:mappings_def Un_def Int_def image_def)
   apply(metis)+
 done
@@ -57,26 +60,11 @@ definition SubstP ::
 
 subsection {* Theorems *}
 
-text {* General Functions *}
-
-theorem bij_comp_inject :
-"bij g \<Longrightarrow> (f1 \<circ> g = f2 \<circ> g) = (f1 = f2)"
-apply (safe)
-apply (rule ext)
-apply (subgoal_tac "\<exists> y . x = g y")
-apply (clarify)
-apply (drule_tac x = "y" in fun_cong)
-apply (auto)
-apply (simp add: bij_def surj_def)
-done
-
-declare bij_imp_bij_inv [simp, intro!]
-
 subsubsection {* Variable Substitution *}
 
-theorem VAR_SUBST_inv [simp] :
+theorem VAR_SUBST_inv [closure] :
 "ss \<in> VAR_SUBST \<Longrightarrow> (inv ss) \<in> VAR_SUBST"
-apply (simp add: VAR_SUBST_def)
+apply (simp add: VAR_SUBST_ON_def)
 apply (safe)
 apply (drule_tac x = "inv ss v" in spec)
 apply (erule subst)
@@ -85,20 +73,45 @@ done
 
 theorem VAR_SUBST_inv_inv [simp] :
 "ss \<in> VAR_SUBST \<Longrightarrow> inv (inv ss) = ss"
-apply (simp add: VAR_SUBST_def)
+apply (simp add: VAR_SUBST_ON_def)
 apply (simp add: inv_inv_eq)
 done
 
 theorem VAR_SUBST_ss_inv [simp] :
 "ss \<in> VAR_SUBST \<Longrightarrow> ss (inv ss x) = x"
-apply (simp add: VAR_SUBST_def)
+apply (simp add: VAR_SUBST_ON_def)
 apply (simp add: surj_f_inv_f bij_def)
 done
 
 theorem VAR_SUBST_inv_ss [simp] :
 "ss \<in> VAR_SUBST \<Longrightarrow> inv ss (ss x) = x"
-apply (simp add: VAR_SUBST_def)
+apply (simp add: VAR_SUBST_ON_def)
 apply (simp add: inv_f_f bij_def)
+done
+
+theorem VAR_SUBST_inv_comp [simp] :
+"ss \<in> VAR_SUBST \<Longrightarrow> inv ss \<circ> ss = id"
+apply (simp add: VAR_SUBST_ON_def)
+apply (simp add: inv_f_f bij_def)
+done
+
+theorem VAR_SUBST_inv_comp' [simp] :
+"ss \<in> VAR_SUBST \<Longrightarrow> ss \<circ> inv ss = id"
+apply (simp add: VAR_SUBST_ON_def)
+apply (simp add: inv_f_f bij_def)
+done
+
+theorem VAR_SUBST_inv_dist [simp] :
+"\<lbrakk> ss1 \<in> VAR_SUBST; ss2 \<in> VAR_SUBST \<rbrakk> \<Longrightarrow> inv (ss1 \<circ> ss2) = inv ss2 \<circ> inv ss1"
+apply(simp add:VAR_SUBST_ON_def bij_def)
+apply (auto)
+apply (metis inj_on_imp_bij_betw o_inv_distrib)
+done
+
+theorem VAR_SUBST_image [simp] :
+"\<lbrakk> ss1 \<in> VAR_SUBST; ss2 \<in> VAR_SUBST \<rbrakk> \<Longrightarrow> ss1 ` ss2 ` a = (ss1 \<circ> ss2) ` a"
+apply (simp add: image_def)
+apply (auto)
 done
 
 theorem VAR_SUBST_image_inv [simp] :
@@ -115,31 +128,31 @@ done
 
 theorem VAR_SUBST_in_image_simp [simp] :
 "\<lbrakk>ss \<in> VAR_SUBST\<rbrakk> \<Longrightarrow> (ss x \<in> ss ` a) = (x \<in> a)"
-apply (simp add: VAR_SUBST_def)
+apply (simp add: VAR_SUBST_ON_def)
 apply (auto simp: bij_def inj_eq)
 done
 
-theorem VAR_SUBST_compose [simp]:
+theorem VAR_SUBST_compose [simp,closure]:
 "\<lbrakk> ss1 \<in> VAR_SUBST ; ss2 \<in> VAR_SUBST \<rbrakk> \<Longrightarrow> (ss1 \<circ> ss2) \<in> VAR_SUBST"
-apply (simp add: VAR_SUBST_def)
+apply (simp add: VAR_SUBST_ON_def)
 apply (auto simp: bij_def)
 apply(simp add:inj_comp)
 apply(metis UNIV_I image_compose)
 done
 
-theorem VAR_SUBST_id [simp]:
-"id \<in> VAR_SUBST"
-  by (simp add:VAR_SUBST_def)
+theorem VAR_SUBST_ON_id [simp,closure]:
+"id \<in> VAR_SUBST_ON a"
+  by (simp add:VAR_SUBST_ON_def)
 
 theorem VAR_SUBSTS_disj_comm [simp]:
 "\<lbrakk> ss1 \<in> VAR_SUBST; ss2 \<in> VAR_SUBST; mappings ss1 \<inter> mappings ss2 = {} \<rbrakk> \<Longrightarrow>
  ss1 \<circ> ss2 = ss2 \<circ> ss1"
-  by (auto intro:disj_mapping_comm simp add:VAR_SUBST_def bij_def)
+  by (auto intro:disj_mapping_comm simp add:VAR_SUBST_ON_def bij_def)
 
-theorem VAR_SUBST_WF_BINDING [simp] :
+theorem VAR_SUBST_WF_BINDING [simp,binding] :
 "\<lbrakk>b \<in> WF_BINDING; ss \<in> VAR_SUBST\<rbrakk> \<Longrightarrow>
  b \<circ> ss \<in> WF_BINDING"
-apply (simp add: VAR_SUBST_def WF_BINDING_def)
+apply (simp add: VAR_SUBST_ON_def WF_BINDING_def)
 apply (safe)
 apply (drule_tac x = "ss v" in spec)
 apply (drule_tac x = "v" in spec)
@@ -148,12 +161,11 @@ done
 
 text {* Binding Substitution *}
 
-theorem SubstB_closure [simp] :
+theorem SubstB_closure [closure] :
 "\<lbrakk>ss \<in> VAR_SUBST;
  b \<in> WF_BINDING\<rbrakk> \<Longrightarrow>
  SubstB ss b \<in> WF_BINDING"
-apply (simp add: SubstB_def)
-done
+  by (auto simp add: SubstB_def binding closure)
 
 theorem SubstsB_inject [simp]:
 "\<lbrakk>b1 \<in> WF_BINDING;
@@ -161,7 +173,7 @@ theorem SubstsB_inject [simp]:
  ss \<in> VAR_SUBST\<rbrakk> \<Longrightarrow>
  (SubstB ss b1 = SubstB ss b2) = (b1 = b2)"
 apply (simp add: SubstB_def)
-apply (simp add: VAR_SUBST_def)
+apply (simp add: VAR_SUBST_ON_def)
 apply (simp add: bij_comp_inject)
 done
 
@@ -170,9 +182,9 @@ theorem SubstB_inv_cancel1 [simp] :
  b \<in> WF_BINDING\<rbrakk> \<Longrightarrow>
  SubstB (inv ss) (SubstB ss b) = b"
 apply (subgoal_tac "SubstB ss b \<in> WF_BINDING")
-apply (simp add: SubstB_def)
+apply (simp add: SubstB_def closure binding)
 apply (rule ext)
-apply (simp_all)
+apply (simp_all add:closure)
 done
 
 theorem SubstB_inv_cancel2 [simp] :
@@ -180,18 +192,18 @@ theorem SubstB_inv_cancel2 [simp] :
  b \<in> WF_BINDING\<rbrakk> \<Longrightarrow>
  SubstB ss (SubstB (inv ss) b) = b"
 apply (subgoal_tac "SubstB (inv ss) b \<in> WF_BINDING")
-apply (simp add: SubstB_def)
+apply (simp add: SubstB_def closure binding)
 apply (rule ext)
-apply (simp_all)
+apply (simp_all add:closure)
 done
 
-theorem SubstB_compose:
+theorem SubstB_compose [simp]:
 "\<lbrakk>ss1 \<in> VAR_SUBST; ss2 \<in> VAR_SUBST;
  b \<in> WF_BINDING\<rbrakk> \<Longrightarrow>
  SubstB ss1 (SubstB ss2 b) = SubstB (ss1\<circ>ss2) b"
 apply(subgoal_tac "SubstB ss2 b \<in> WF_BINDING")
 apply(simp add: SubstB_def)
-apply(auto simp add:VAR_SUBST_def o_inv_distrib)
+apply(auto simp add:VAR_SUBST_ON_def o_inv_distrib closure)
 done
 
 theorem SubstB_id [simp] :
@@ -221,17 +233,17 @@ lemma SubstB_override2:
 "\<lbrakk> ss \<in> VAR_SUBST; a \<in> WF_ALPHABET;
    b \<in> WF_BINDING; b' \<in> WF_BINDING \<rbrakk> \<Longrightarrow>
 SubstB (inv ss) (SubstB ss b \<oplus> b' on ss ` a) = b \<oplus> SubstB (inv ss) b' on a"
-apply (simp add:SubstB_def)
+apply (simp add:SubstB_def closure binding)
 apply (simp add:override_on_def)
-apply(rule ext)
-apply(auto)
+apply (rule ext)
+apply (auto)
 done
 
 lemma SubstB_override3:
 "\<lbrakk> ss \<in> VAR_SUBST; a \<in> WF_ALPHABET;
    b \<in> WF_BINDING; b' \<in> WF_BINDING; mappings ss \<inter> a = {} \<rbrakk> \<Longrightarrow>
 SubstB ss (b \<oplus> b' on a) = (SubstB ss b) \<oplus> (SubstB ss b') on a"
-apply(simp add:SubstB_def)
+apply(simp add:SubstB_def closure binding)
 apply(simp add:override_on_def)
 apply(rule ext)
 apply(auto)
@@ -244,13 +256,53 @@ lemma SubstB_override4:
 "\<lbrakk> ss \<in> VAR_SUBST; a \<in> WF_ALPHABET;
    b \<in> WF_BINDING; b' \<in> WF_BINDING; mappings ss \<inter> a = {} \<rbrakk> \<Longrightarrow>
 SubstB ss (b \<oplus> b' on a) = SubstB ss (b \<oplus> (SubstB ss b') on a)"
-apply(simp add:SubstB_def)
+apply(simp add:SubstB_def closure binding)
 apply(simp add:override_on_def)
 apply(rule ext)
 apply(auto)
 apply(simp add:mappings_def Un_def Int_def)
 apply(metis)
 done
+
+lemma override_id_bij:
+  assumes "ss \<in> VAR_SUBST_ON a" "a \<in> WF_ALPHABET"
+  shows "bij (id \<oplus> ss on a)"
+proof -
+  have "bij_betw (id \<oplus> ss on a) UNIV UNIV = bij_betw (id \<oplus> ss on a) (a \<union> (-a)) (a \<union> (-a))"
+    by (metis sup_compl_top)
+
+  moreover from assms have "bij_betw (id \<oplus> ss on a) (a \<union> (-a)) (a \<union> (-a))"
+    by (rule_tac override_bij, auto simp add:VAR_SUBST_ON_def)
+  
+  ultimately show ?thesis
+    by auto
+qed    
+
+lemma SubstB_override5: 
+  assumes "ss \<in> VAR_SUBST_ON a1" "a1 \<in> WF_ALPHABET" "a2 \<in> WF_ALPHABET"
+          "a1 \<inter> a2 = {}" "b \<in> WF_BINDING"
+  shows   "(SubstB (id \<oplus> ss on a1) b) \<cong> b on a2"
+proof -
+  from assms have "bij_betw (id \<oplus> ss on a1) UNIV UNIV"
+    by (metis override_id_bij)
+
+  with assms have "id \<oplus> ss on a1 \<in> VAR_SUBST"
+    apply(auto simp add:VAR_SUBST_ON_def)
+    by (metis id_def override_on_def) 
+
+  moreover from assms have "bij_split ss a1 a1"
+    by (simp add:VAR_SUBST_ON_def)
+
+  moreover from assms have "bij_split id a2 a2"
+    by simp
+
+  ultimately show ?thesis using assms
+    apply(simp add:SubstB_def beta_equiv_def override_inv_id)
+    apply(auto)
+    apply(simp add:override_on_def)
+    apply(force)
+  done
+qed
 
 lemma SubstB_invol:
 "\<lbrakk> ss \<in> VAR_SUBST; b \<in> WF_BINDING; ss \<circ> ss = id \<rbrakk> \<Longrightarrow>
@@ -259,19 +311,24 @@ lemma SubstB_invol:
 
 subsubsection {* Predicate Substitution *}
 
-theorem SubstP_alphabet [simp] :
+theorem SubstP_alphabet [alphabet] :
 "\<lbrakk>p \<in> WF_ALPHA_PREDICATE;
  ss \<in> VAR_SUBST\<rbrakk> \<Longrightarrow>
  \<alpha> p[ss] = ss ` (\<alpha> p)"
-apply (simp add: SubstP_def)
+  by (simp add: SubstP_def)
+
+lemma [alphabet]: "ss \<in> VAR_SUBST \<Longrightarrow> inv ss ` ss ` a = a"
+  by (auto simp add:bij_def)
+
+lemma [alphabet]: "ss \<in> VAR_SUBST \<Longrightarrow> ss ` (a - b) = ss ` a - ss ` b"
+  apply (simp add:bij_def VAR_SUBST_ON_def inj_on_def var)
+  apply(auto)
 done
 
-(*
-theorem SubstP_alpha_disj_comm [simp] :
-"\<lbrakk>p \<in> WF_ALPHA_PREDICATE;
- ss1 \<in> VAR_SUBST; ss2 \<in> VAR_SUBST; 
- mappings ss1 \<inter> mappings ss2 = {} \<rbrakk> \<Longrightarrow>
-*)
+lemma WF_ALPHABET_image_subst[alphabet]: "\<lbrakk> a \<in> WF_ALPHABET; ss \<in> VAR_SUBST \<rbrakk> \<Longrightarrow> ss ` a \<in> WF_ALPHABET"
+  apply(simp only:VAR_SUBST_ON_def)
+  apply(auto simp add:bij_def WF_ALPHABET_def)
+done
 
 text {* Could the following be useful in other places too? Examine! *}
 
@@ -281,15 +338,15 @@ theorem SubstP_closure_lemma :
  b2 \<in> WF_BINDING\<rbrakk> \<Longrightarrow>
  SubstB ss b1 \<cong> b2 on ss ` a \<longrightarrow> b1 \<cong> SubstB (inv ss) b2 on a"
 apply (simp add: beta_equiv_def)
-apply (simp add: SubstB_def)
+apply (simp add: SubstB_def closure)
 done
 
-theorem SubstP_closure [simp] :
+theorem SubstP_closure [closure] :
 "\<lbrakk>p \<in> WF_ALPHA_PREDICATE;
  ss \<in> VAR_SUBST\<rbrakk> \<Longrightarrow>
  p[ss] \<in> WF_ALPHA_PREDICATE"
 apply (simp add: SubstP_def)
-apply (simp add: WF_ALPHA_PREDICATE_def)
+apply (simp only: WF_ALPHA_PREDICATE_def)
 apply (safe)
 -- {* Subgoal 1 *}
 apply (auto simp: WF_ALPHABET_def)
@@ -298,7 +355,7 @@ apply (simp add: WF_BINDING_SET_def)
 apply (safe)
 -- {* Subgoal 2.1 *}
 apply (subgoal_tac "xa \<in> WF_BINDING")
-apply (simp)
+apply (simp add:closure)
 apply (auto) [1]
 -- {* Subgoal 2.2 *}
 apply (simp (no_asm_simp) add: image_def)
@@ -307,7 +364,7 @@ apply (simp)
 apply (drule_tac x = "b1" in bspec)
 apply (assumption)
 apply (drule_tac x = "SubstB (inv ss) b2" in bspec)
-apply (simp)
+apply (simp add:closure)
 apply (subgoal_tac "b1 \<cong> SubstB (inv ss) b2 on \<alpha> p")
 apply (simp)
 apply (subst SubstP_closure_lemma)
@@ -319,7 +376,7 @@ theorem EvalP_SubstP [eval] :
  ss \<in> VAR_SUBST;
  b \<in> WF_BINDING\<rbrakk> \<Longrightarrow>
  EvalP p[ss] b = EvalP p (SubstB (inv ss) b)"
-apply (simp add: EvalP_def)
+apply (simp add: EvalP_def closure)
 apply (simp add: SubstP_def)
 apply (simp add: image_def)
 apply (safe)
@@ -336,7 +393,7 @@ theorem EvalP_SubstsP_SubstB [simp] :
  b \<in> WF_BINDING;
  ss \<in> VAR_SUBST\<rbrakk> \<Longrightarrow>
  EvalP p[ss] (SubstB ss b) = EvalP p b"
-apply (simp add: EvalP_def)
+apply (simp add: EvalP_def closure)
 apply (simp add: SubstP_def)
 apply (simp add: image_def)
 apply (auto)
@@ -351,87 +408,83 @@ theorem SubstP_inverse :
 "\<lbrakk>p \<in> WF_ALPHA_PREDICATE;
  ss \<in> VAR_SUBST\<rbrakk> \<Longrightarrow>
  p[ss][inv ss] = p"
-apply (utp_pred_taut_tac)
-done
+  by (utp_pred_eq_tac2)
 
 theorem SubstP_compose :
 "\<lbrakk>p \<in> WF_ALPHA_PREDICATE;
  ss1 \<in> VAR_SUBST; ss2 \<in> VAR_SUBST\<rbrakk> \<Longrightarrow>
  p[ss1][ss2] = p[ss2\<circ>ss1]"
-apply (utp_pred_eq_tac)
-apply(rule conjI)
-apply(force)
-apply(simp add:SubstB_compose)
-apply(simp add:o_inv_distrib VAR_SUBST_def)
-done
+  by (utp_pred_eq_tac2)
 
 theorem SubstP_disj_comm:
 "\<lbrakk> p \<in> WF_ALPHA_PREDICATE; ss1 \<in> VAR_SUBST; ss2 \<in> VAR_SUBST
 ; mappings ss1 \<inter> mappings ss2 = {} \<rbrakk> \<Longrightarrow> p[ss1][ss2] = p[ss2][ss1]"
-apply (utp_pred_eq_tac)
-apply(rule conjI)
-apply(metis SubstP_alphabet SubstP_closure SubstP_compose VAR_SUBSTS_disj_comm)
-apply(smt SubstB_closure SubstB_def SubstB_disj_comm SubstB_inv_cancel2 SubstsB_inject VAR_SUBST_inv VAR_SUBST_inv_inv)
+apply (rule eval_intro)
+apply (blast intro:closure alpha_closure)
+apply (blast intro:closure alpha_closure)
+apply (simp add:closure alphabet)
+apply (metis VAR_SUBSTS_disj_comm)
+apply (simp add:eval closure)
+apply (metis VAR_SUBSTS_disj_comm VAR_SUBST_inv_dist)
 done
 
 theorem SubstP_id :
-"\<lbrakk>p \<in> WF_ALPHA_PREDICATE \<rbrakk> \<Longrightarrow>
+"\<lbrakk> p \<in> WF_ALPHA_PREDICATE \<rbrakk> \<Longrightarrow>
  p[id] = p"
-  by (utp_pred_eq_tac)
+  by (utp_pred_eq_tac2)
+
+lemma SubstP_invol:
+"\<lbrakk> ss \<in> VAR_SUBST; p \<in> WF_ALPHA_PREDICATE; ss \<circ> ss = id \<rbrakk> \<Longrightarrow>
+ p[ss][ss] = p"
+  by (metis SubstP_compose SubstP_id)
 
 theorem SubstP_AndP_distr :
 "\<lbrakk>p1 \<in> WF_ALPHA_PREDICATE;
  p2 \<in> WF_ALPHA_PREDICATE;
  ss \<in> VAR_SUBST\<rbrakk> \<Longrightarrow>
  (p1 \<and>p p2)[ss] = p1[ss] \<and>p p2[ss]"
-apply (utp_pred_eq_tac)
-apply (auto)
-done
+  by (utp_pred_eq_tac2)
 
 theorem SubstP_OrP_distr :
 "\<lbrakk>p1 \<in> WF_ALPHA_PREDICATE;
  p2 \<in> WF_ALPHA_PREDICATE;
  ss \<in> VAR_SUBST\<rbrakk> \<Longrightarrow>
  (p1 \<or>p p2)[ss] = p1[ss] \<or>p p2[ss]"
-apply (utp_pred_eq_tac)
-apply (auto)
-done
+  by (utp_pred_eq_tac2)
 
 theorem SubstP_NotP_distr :
 "\<lbrakk>p \<in> WF_ALPHA_PREDICATE;
  ss \<in> VAR_SUBST\<rbrakk> \<Longrightarrow>
  (\<not>p p)[ss] = \<not>p p[ss]"
-apply (utp_pred_eq_tac)
-done
+  by (utp_pred_eq_tac2)
 
 theorem ExistsResP_Subst:
 "\<lbrakk>p \<in> WF_ALPHA_PREDICATE;
   ss \<in> VAR_SUBST; a \<in> WF_ALPHABET \<rbrakk> \<Longrightarrow>
   p \<ominus>p a = (p[ss] \<ominus>p (ss ` a))[inv ss]"
-apply (utp_pred_eq_tac)
-apply(rule conjI)
-apply (smt VAR_SUBST_image_inv VAR_SUBST_inv VAR_SUBST_inv_inv image_diff_subset image_mono set_eq_subset)
+apply(utp_pred_eq_tac2)
 apply(auto)
 apply(rule_tac x="SubstB ss b'" in bexI)
-apply(auto simp add:SubstB_override1)
+apply(auto simp add:SubstB_override1 closure)
 apply(rule_tac x="SubstB (inv ss) b'" in bexI)
-apply(auto simp add:SubstB_override2)
+apply(auto simp add:SubstB_override2 closure)
 done
 
 theorem ResP_Subst_disj:
   assumes "p \<in> WF_ALPHA_PREDICATE" "ss \<in> VAR_SUBST" "a \<in> WF_ALPHABET" "mappings ss \<inter> a = {}"
   shows "(p \<ominus>p a)[ss] = p[ss] \<ominus>p a"
 apply(insert assms)
-apply(utp_pred_eq_tac)
-apply(rule conjI)
-apply(simp add:VAR_SUBST_def bij_def image_set_diff disj_mapping_image)
-apply(auto)
+apply(simp add:eval closure alphabet)
+apply(rule ballI)
+apply(rule iffI)
+apply(erule bexE)
 apply(rule_tac x="SubstB (inv ss) b'" in bexI)
 apply (smt SubstB_closure SubstB_inv_cancel2 SubstB_override3 SubstB_override4 VAR_SUBST_inv VAR_SUBST_inv_inv WF_BINDING_override)
-apply(force)
+apply(simp add:closure)
+apply(erule bexE)
 apply(rule_tac x="SubstB (inv ss) b'" in bexI)
 apply (smt SubstB_closure SubstB_inv_cancel2 SubstB_override2 VAR_SUBST_inv assms(2) disj_mapping_image)
-apply(force)
+apply(simp add:closure)
 done
 
 theorem ExistsResP_Subst_disj:
@@ -439,7 +492,7 @@ theorem ExistsResP_Subst_disj:
   shows "(\<exists>-p a . p)[ss] = (\<exists>-p a . p[ss])"
 apply(insert assms)
 apply(simp add:ExistsResP_def)
-apply(simp add:ResP_Subst_disj)
+apply(simp add:ResP_Subst_disj alphabet closure eval)
 done
 
 (*
@@ -453,27 +506,30 @@ apply(utp_pred_eq_tac)
 apply(auto)
 *)
 
+
+lemma [simp]:"ss \<in> VAR_SUBST \<Longrightarrow> bij ss"
+  by (simp add:VAR_SUBST_ON_def)
+
+lemma [simp]:"ss \<in> VAR_SUBST \<Longrightarrow> inj ss"
+  by (simp add:VAR_SUBST_ON_def bij_def)
+
+lemma [simp]:"ss \<in> VAR_SUBST \<Longrightarrow> surj ss"
+  apply(simp only:VAR_SUBST_ON_def)
+  apply(auto simp add:bij_def)
+done
+
+
 theorem Closure_SubstP :
 "\<lbrakk>p \<in> WF_ALPHA_PREDICATE;
  ss \<in> VAR_SUBST\<rbrakk> \<Longrightarrow>
  [p[ss]] = ([p] :: ('VALUE, 'TYPE) ALPHA_PREDICATE)"
-apply (utp_pred_taut_tac)
+apply(utp_pred_eq_tac2)
 apply (auto)
 -- {* Can we automate discharging the following residual subgoal? *}
 apply (drule_tac x = "SubstB ss x" in bspec)
-apply (simp)
-apply (simp add: SubstB_def)
-apply (subgoal_tac
-  "EvalP p (((b \<oplus> (x \<circ> (inv ss)) on ss ` \<alpha> p) \<circ> ss) \<oplus> x on - \<alpha> p)")
-apply (subgoal_tac
-  "x = ((b \<oplus> (x \<circ> (inv ss)) on ss ` \<alpha> p) \<circ> ss) \<oplus> x on - \<alpha> p")
-apply (simp)
-apply (rule ext)
-apply (simp add: comp_def)
-apply (case_tac "ss xa \<in> ss ` \<alpha> p")
-apply (simp)
-apply (simp)
-apply (simp_all add: EvalP_override)
+apply (simp add:closure override_before binding)
+apply (simp add: SubstB_def override_before closure binding bij_def)
+apply (simp add: SubstB_def override_before closure binding bij_def)
 done
 
 subsection {* Proof Experiments *}
@@ -484,17 +540,154 @@ text {*
   the strategy alone is not powerful enough to prove the theorem by itself.
 *}
 
+declare bij_comp_inject [alphabet]
+
+
 theorem SubstP_lemma1 :
 "\<lbrakk>p1 \<in> WF_ALPHA_PREDICATE;
  p2 \<in> WF_ALPHA_PREDICATE;
  ss \<in> VAR_SUBST\<rbrakk> \<Longrightarrow>
  taut [p1 \<Leftrightarrow>p p2] \<Leftrightarrow>p [p1[ss] \<Leftrightarrow>p p2[ss]]"
-apply (subgoal_tac "p1[ss] \<Leftrightarrow>p p2[ss] = (p1 \<Leftrightarrow>p p2)[ss]")
-apply (simp)
-apply (simp add: Closure_SubstP)
-apply (utp_pred_taut_tac)
-apply (utp_pred_eq_tac)
-apply (auto)
+apply(auto intro!:eval_intro simp add:closure eval SubstB_def binding)
+apply(erule_tac x="b' \<circ> inv ss" in ballE, (simp add:binding closure)+)+
 done
+
+lemma VAR_SUBST_ON_subset:
+"\<lbrakk> ss \<in> VAR_SUBST_ON a; b \<subseteq> a \<rbrakk> \<Longrightarrow> ss ` b \<subseteq> a"
+  by (auto simp add:VAR_SUBST_ON_def image_def bij_betw_def)
+
+lemma VAR_SUBST_ON_override_id[closure]: 
+  assumes "a \<in> WF_ALPHABET" "ss \<in> VAR_SUBST_ON a"
+  shows "id \<oplus> ss on a \<in> VAR_SUBST"
+apply(insert assms)
+apply(simp only:VAR_SUBST_ON_def)
+apply(auto)
+apply (metis assms(2) override_id_bij)
+apply(simp add:override_on_def)
+done
+
+(*
+theorem VAR_SUBST_ON_override:
+"\<lbrakk> ss1 \<in> VAR_SUBST_ON a; ss2 \<in> VAR_SUBST_ON b; a \<inter> b = {} \<rbrakk> \<Longrightarrow> ss1 \<oplus> ss2 on b \<in> VAR_SUBST_ON (a \<union> b)"
+proof (simp add:VAR_SUBST_ON_def, safe)
+  assume assm:"a \<inter> b = {}" "bij_betw ss1 a a" "bij_betw ss2 b b"
+
+  thus "bij_betw (ss1 \<oplus> ss2 on b) (a \<union> b) (a \<union> b)"
+  proof -
+    from assm have "inj_on (ss1 \<oplus> ss2 on b) (a \<union> b)"
+      apply(simp add:inj_on_def bij_betw_def override_on_def)
+      apply(metis IntI UnE emptyE imageI)
+    done
+
+    moreover
+    from assm have "(ss1 \<oplus> ss2 on b) ` a  = a"
+      by (metis bij_betw_def inf_commute override_imageL)
+
+    moreover
+    from assm have "(ss1 \<oplus> ss2 on b) ` b  = b"
+      by (metis bij_betw_def override_imageR)
+
+    ultimately show ?thesis
+      by (auto simp add:bij_betw_def)
+  qed
+next
+  fix v
+  assume assm: "\<forall>v\<in>a. type (ss1 v) = type v" "\<forall>v\<in>b. type (ss2 v) = type v" "v \<in> a"
+  thus "type ((ss1 \<oplus> ss2 on b) v) = type v"
+    by (simp add:override_on_def)
+next
+  fix v
+  assume assm: "\<forall>v\<in>a. type (ss1 v) = type v" "\<forall>v\<in>b. type (ss2 v) = type v" "v \<in> b"
+  thus "type ((ss1 \<oplus> ss2 on b) v) = type v"
+    by (simp add:override_on_def)
+next
+  assume assm:"a \<inter> b = {}" "bij_betw ss1 (a) (a)" "bij_betw ss2 (b) (b)" "bij_betw ss1 (-a) (-a)" "bij_betw ss2 (-b) (-b)"
+
+
+  thus "bij_betw (ss1 \<oplus> ss2 on b) (- a \<inter> - b) (- a \<inter> - b)"
+    
+    apply(simp add: override_on_def bij_betw_def inj_on_def)
+    apply(blast)
+    apply(auto)
+    apply(case_tac "xa \<in> (-a)")
+   
+    apply(force)
+    sorry
+qed
+*)
+
+lemma [simp]: "ss \<in> VAR_SUBST \<Longrightarrow> ss ` (a \<inter> b) \<subseteq> ss ` a"
+  by (unfold VAR_SUBST_ON_def, auto simp add: bij_def)
+
+lemma VAR_SUBST_image_inter[simp]: "ss \<in> VAR_SUBST \<Longrightarrow> ss ` (a \<inter> b) = ss ` a \<inter> ss ` b"
+  by (unfold VAR_SUBST_ON_def, auto simp add:bij_def inj_on_def)
+
+theorem ResP_image:
+  assumes "p \<in> WF_ALPHA_PREDICATE" "a \<in> WF_ALPHABET" "ss \<in> VAR_SUBST_ON a"
+  shows "p \<ominus>p a = p [id \<oplus> ss on a] \<ominus>p (ss ` a)"
+apply(insert assms)
+apply(utp_pred_eq_tac2)
+apply(simp only:VAR_SUBST_ON_def bij_split_def bij_betw_def)
+apply(blast)
+apply(simp add:eval closure alpha_closure)
+apply(rule_tac ballI)
+apply(simp add:eval alphabet closure var SubstB_def)
+apply(auto)
+sorry
+
+
+lemma [alphabet]: "ss \<in> VAR_SUBST_ON a \<Longrightarrow> bij_betw ss a a"
+  by (simp add:VAR_SUBST_ON_def)
+
+theorem ExistsResP_image:
+  assumes "p \<in> WF_ALPHA_PREDICATE" "a \<in> WF_ALPHABET" "ss \<in> VAR_SUBST_ON a"
+  shows "(\<exists>-p a . p) = (\<exists>-p a . p [id \<oplus> ss on a])"
+  apply (insert assms)
+  apply (rule EqualityP_intro)
+  apply (simp_all add:closure alphabet var)
+  apply (auto)[1]
+  apply (force simp add:VAR_SUBST_ON_def bij_betw_def)
+  apply (auto simp add:closure alphabet var eval)
+  apply (auto simp add:SubstB_def closure)
+
+  sorry
+
+(*
+proof -
+  from assms have "(\<exists>-p a . p) = (\<exists>-p ss ` a . p [id \<oplus> ss on a])"
+    by (metis assms ExistsResP_def ResP_image SubstP_closure VAR_SUBST_ON_override_id WF_ALPHABET_image)
+
+  also from assms have "... = (\<exists>-p a . p [id \<oplus> ss on a])"
+    by (simp add:VAR_SUBST_ON_def bij_betw_def)
+
+  finally show ?thesis .
+qed
+*)
+
+theorem ExistsResP_intrude:
+  assumes "p \<in> WF_ALPHA_PREDICATE" "a \<in> WF_ALPHABET" "ss \<in> VAR_SUBST"
+  shows "(\<exists>-p a . p)[ss] = (\<exists>-p (ss ` a) . p[ss])"
+apply(insert assms)
+apply(utp_pred_eq_tac2)
+apply(auto simp add:SubstB_def closure)
+apply(rule_tac x="b' \<circ> inv ss" in bexI)
+apply(auto simp add:closure)
+done
+
+inductive_set gen_pred :: "(('VALUE, 'TYPE) ALPHA_PREDICATE) set" where
+  "a \<in> WF_ALPHABET \<Longrightarrow> true a \<in> gen_pred"  |
+  "a \<in> WF_ALPHABET \<Longrightarrow> false a \<in> gen_pred" |
+  "\<lbrakk> p \<in> gen_pred; q \<in> gen_pred \<rbrakk> \<Longrightarrow> p \<and>p q \<in> gen_pred" |
+  "\<lbrakk> p \<in> gen_pred; q \<in> gen_pred \<rbrakk> \<Longrightarrow> p \<or>p q \<in> gen_pred" |
+  "p \<in> gen_pred \<Longrightarrow> \<not>p p \<in> gen_pred"
+
+print_theorems
+
+lemma "gen_pred \<subseteq> WF_ALPHA_PREDICATE"
+apply(clarify)
+apply(erule gen_pred.induct)
+apply(auto)
+sorry 
+
 end
 end
