theories/generic/utp_alphabet.thy
@@ -10,7 +10,24 @@ theory utp_alphabet
 imports utp_var
 begin
 
-types 'TYPE ALPHABET = "'TYPE VAR set"
+type_synonym 'TYPE ALPHABET = "'TYPE VAR set"
+
+text {* Create a theorem set for alphabets *}
+
+ML {*
+  structure AlphabetThm =
+    Named_Thms (val name = @{binding "alphabet"} val description = "alphabet theorems");
+*}
+
+setup {* AlphabetThm.setup *}
+
+ML {*
+  structure AlphaClosureThm =
+    Named_Thms (val name = @{binding "alpha_closure"} val description = "alphabet closure theorems");
+*}
+
+setup {* AlphaClosureThm.setup *}
+
 
 context VAR
 begin
@@ -64,69 +81,59 @@ subsection {* Theorems *}
 
 subsubsection {* Closure Theorems *}
 
-theorem WF_ALPHABET_empty [simp] :
+theorem WF_ALPHABET_empty [alpha_closure] :
 "{} \<in> WF_ALPHABET"
-apply (simp add: WF_ALPHABET_def)
-done
+  by (simp add: WF_ALPHABET_def)
 
-theorem WF_ALPHABET_insert [simp] :
+theorem WF_ALPHABET_insert [alpha_closure] :
 "\<lbrakk>a \<in> WF_ALPHABET\<rbrakk> \<Longrightarrow>
  (insert x a) \<in> WF_ALPHABET"
-apply (simp add: WF_ALPHABET_def)
-done
+  by (simp add: WF_ALPHABET_def)
 
-theorem WF_ALPHABET_union [intro,simp] :
+theorem WF_ALPHABET_union [alpha_closure] :
 "\<lbrakk>a1 \<in> WF_ALPHABET;
  a2 \<in> WF_ALPHABET\<rbrakk> \<Longrightarrow>
  a1 \<union> a2 \<in> WF_ALPHABET"
-apply (simp add: WF_ALPHABET_def)
-done
+  by (simp add: WF_ALPHABET_def)
 
-theorem WF_ALPHABET_inter [intro,simp] :
+theorem WF_ALPHABET_inter [alpha_closure] :
 "\<lbrakk>a1 \<in> WF_ALPHABET;
  a2 \<in> WF_ALPHABET\<rbrakk> \<Longrightarrow>
  a1 \<inter> a2 \<in> WF_ALPHABET"
-apply (simp add: WF_ALPHABET_def)
-done
+  by (simp add: WF_ALPHABET_def)
 
-theorem WF_ALPHABET_diff [intro,simp] :
+theorem WF_ALPHABET_diff [alpha_closure] :
 "\<lbrakk>a1 \<in> WF_ALPHABET;
  a2 \<in> WF_ALPHABET\<rbrakk> \<Longrightarrow>
  a1 - a2 \<in> WF_ALPHABET"
-apply (simp add: WF_ALPHABET_def)
-done
+  by (simp add: WF_ALPHABET_def)
 
-theorem WF_ALPHABET_subset [intro] :
+text {* This lemma can really slow down the simplifier, handle with care. *}
+
+theorem WF_ALPHABET_subset [intro]:
 "\<lbrakk>a \<in> WF_ALPHABET; b \<subseteq> a\<rbrakk> \<Longrightarrow>
  b \<in> WF_ALPHABET"
-apply (simp add: WF_ALPHABET_def)
-apply (simp add: finite_subset)
-done
+  by (simp add: WF_ALPHABET_def finite_subset)
 
-theorem WF_ALPHABET_image [simp] :
+theorem WF_ALPHABET_image [alpha_closure] :
 "\<lbrakk>a \<in> WF_ALPHABET\<rbrakk> \<Longrightarrow>
  f ` a \<in> WF_ALPHABET"
-apply (simp add: WF_ALPHABET_def)
-done
+  by (simp add: WF_ALPHABET_def)
 
-theorem WF_ALPHABET_in [simp, intro] :
+theorem WF_ALPHABET_in [alpha_closure] :
 "a \<in> WF_ALPHABET \<Longrightarrow>
  in a \<in> WF_ALPHABET"
-apply (simp add: in_alphabet_def)
-apply (simp add: WF_ALPHABET_def)
-done
+  by (simp add: in_alphabet_def WF_ALPHABET_def)
 
-theorem WF_ALPHABET_out [simp, intro] :
+theorem WF_ALPHABET_out [alpha_closure] :
 "a \<in> WF_ALPHABET \<Longrightarrow>
  out a \<in> WF_ALPHABET"
-apply (simp add: out_alphabet_def)
-apply (simp add: WF_ALPHABET_def)
-done
+  by (simp add: out_alphabet_def WF_ALPHABET_def)
 
-theorem WF_ALPHABET_homalph [simp, intro] :
+theorem WF_ALPHABET_homalph [alpha_closure] :
 "a \<in> WF_ALPHABET \<Longrightarrow>
  homalph a \<in> WF_ALPHABET"
-  by (simp add: homalph_def)
+  by (auto intro:alpha_closure simp add:homalph_def)
 
 subsection {* Simon's Theorems *}
 
@@ -135,122 +142,88 @@ theorem COMPOSABLE_intro [intro!] :
  b \<in> WF_ALPHABET;
  out a = dash ` in b\<rbrakk> \<Longrightarrow>
  COMPOSABLE a b"
-apply (auto simp: utp_alphabet_simps)
-done
+  by (auto simp: utp_alphabet_simps)
 
 theorem COMPOSABLE_elim [elim] :
 "\<lbrakk>COMPOSABLE a b;
  a \<in> WF_ALPHABET;
  b \<in> WF_ALPHABET;
  out a = dash ` in b \<Longrightarrow> P\<rbrakk> \<Longrightarrow> P"
-apply (auto simp: utp_alphabet_simps)
-done
+  by (auto simp: utp_alphabet_simps)
 
 theorem COMPOSABLE_dest [dest] :
 "\<lbrakk>COMPOSABLE a b;
  a \<in> WF_ALPHABET;
  b \<in> WF_ALPHABET\<rbrakk> \<Longrightarrow>
  out a = dash ` in b"
-apply (auto simp: utp_alphabet_simps)
-done
+  by (auto simp: utp_alphabet_simps)
 
-theorem in_alphabet_in [simp] :
+theorem in_alphabet_in [var] :
 "in (in a) = in a"
-apply (auto simp: utp_alphabet_simps)
-done
+  by (auto simp add: in_alphabet_def)
 
-theorem in_alphabet_out [simp] :
+theorem in_alphabet_out [var] :
 "in (out a) = {}"
-apply (auto simp: utp_alphabet_simps)
-done
+  by (auto simp: utp_alphabet_simps)
 
-theorem out_alphabet_out [simp] :
+theorem out_alphabet_out [var] :
 "out (out a) = out a"
-apply (auto simp: utp_alphabet_simps)
-done
+  by (auto simp: utp_alphabet_simps)
 
-theorem out_alphabet_in [simp] :
+theorem out_alphabet_in [var] :
 "out (in a) = {}"
-apply (auto simp: utp_alphabet_simps)
-done
+  by (auto simp: utp_alphabet_simps)
 
-theorem in_alphabet_union [simp] :
+theorem in_alphabet_union [var] :
 "in (a \<union> b) = in a \<union> in b"
-apply (auto simp: utp_alphabet_simps)
-done
+  by (auto simp: utp_alphabet_simps)
 
-theorem out_alphabet_union [simp] :
+theorem out_alphabet_union [var] :
 "out (a \<union> b) = out a \<union> out b"
-by (auto simp: utp_alphabet_simps)
+  by (auto simp: utp_alphabet_simps)
 
-theorem in_alphabet_ndash [simp] :
+theorem in_alphabet_ndash [var] :
 "dash x \<notin> in a"
-by (simp add:utp_alphabet_simps dash_def)
+  by (simp add:utp_alphabet_simps dash_def)
 
-theorem out_alphabet_ndash [simp] : 
+theorem out_alphabet_ndash [var] : 
 "x \<in> out a \<Longrightarrow> dash x \<notin> out b"
-by (simp add:utp_alphabet_simps dash_def)
+  by (simp add:utp_alphabet_simps dash_def)
 
-theorem in_undashed [simp]:
+theorem in_undashed [var]:
 "in a \<subseteq> UNDASHED"
   by (simp add: UNDASHED_def in_alphabet_def)
 
-theorem out_undashed [simp]:
+theorem out_undashed [var]:
 "out a \<subseteq> DASHED"
   by (simp add: DASHED_def out_alphabet_def)
 
-theorem dash_undashed [simp]:
-"a \<subseteq> UNDASHED \<Longrightarrow> dash ` a \<subseteq> DASHED"
-  by (auto simp add: DASHED_def UNDASHED_def dash_def)
-
-theorem dash_dashed [simp]:
-"a \<subseteq> DASHED \<Longrightarrow> dash ` a \<subseteq> DASHED_TWICE"
-  by (auto simp add: DASHED_def DASHED_TWICE_def dash_def)
-
-theorem undash_dashed [simp]:
-"a \<subseteq> DASHED \<Longrightarrow> undash ` a \<subseteq> UNDASHED"
-  by (auto simp add: DASHED_def UNDASHED_def undash_def)
-
-theorem undash_dashed_twice [simp]:
-"a \<subseteq> DASHED_TWICE \<Longrightarrow> undash ` a \<subseteq> DASHED"
-  by (auto simp add: DASHED_def DASHED_TWICE_def undash_def)
-
-lemma out_undash: "a \<subseteq> UNDASHED \<union> DASHED \<Longrightarrow> out (undash ` a) = {}"
+lemma out_undash[var]: "a \<subseteq> UNDASHED \<union> DASHED \<Longrightarrow> out (undash ` a) = {}"
   by (auto simp add:utp_alphabet_simps image_def undash_def)
  
-lemma in_undash:"a \<subseteq> UNDASHED \<union> DASHED \<Longrightarrow> in (undash ` a) = undash ` a"
+lemma in_undash[var]:"a \<subseteq> UNDASHED \<union> DASHED \<Longrightarrow> in (undash ` a) = undash ` a"
   by (auto simp add:utp_alphabet_simps undash_def image_def)
 
-lemma in_dash: "in (dash ` a) = {}"
+lemma in_dash[var]: "in (dash ` a) = {}"
   by (auto simp add:utp_alphabet_simps dash_def image_def)
 
-lemma out_undash_out: "out (undash ` out a) = {}"
+lemma out_undash_out[var]: "out (undash ` out a) = {}"
   by (auto simp add:utp_alphabet_simps undash_def image_def)
 
-lemma out_dash_in: "out (dash ` in a) = dash ` in a"
+lemma out_dash_in[var]: "out (dash ` in a) = dash ` in a"
   by (auto simp add:utp_alphabet_simps dash_def image_def)
-
-theorem dash_undash[simp]: "dashes (name x) > 0 \<Longrightarrow> dash (undash x) = x"
-  apply(auto simp add:dash_def undash_def)
-  apply(smt NAME.surjective pair_collapse unit.exhaust)
-done
-
-theorem undash_dash[simp]: "undash (dash x) = x"
-  apply(auto simp add:dash_def undash_def)
-  apply(smt NAME.surjective pair_collapse unit.exhaust)
-done
   
-lemma dash_undash_out: "dash ` undash ` out a = out a"
-  by (auto simp add:utp_alphabet_simps image_def)
+lemma dash_undash_out[var]: "dash ` undash ` out a = out a"
+  by (auto simp add:utp_alphabet_simps var image_def)
 
-lemma undash_dash' : "undash ` dash ` a = a"
-  by (auto simp add:utp_alphabet_simps image_def)
+lemma undash_dash'[var]: "undash ` dash ` a = a"
+  by (auto simp add:utp_alphabet_simps var image_def)
 
-lemma in_out_disj[simp]: "in a \<inter> out b = {}"
-  by (auto simp add:in_alphabet_def out_alphabet_def DASHED_def UNDASHED_def)
+lemma in_out_disj[var]: "in a \<inter> out b = {}"
+  by (auto simp add:in_alphabet_def var out_alphabet_def DASHED_def UNDASHED_def)
 
-lemma in_out_complete: "a \<subseteq> UNDASHED \<union> DASHED \<Longrightarrow> in a \<union> out a = a"
-  by (auto simp add:utp_alphabet_simps)
+lemma in_out_complete[var]: "a \<subseteq> UNDASHED \<union> DASHED \<Longrightarrow> in a \<union> out a = a"
+  by (auto simp add:utp_alphabet_simps var)
 
 lemma override_out_in: "f \<oplus> (g \<oplus> h on (out a)) on (in b) = f \<oplus> g on (in b)"
   by (metis Diff_triv in_out_disj override_on_cancel4)
@@ -258,35 +231,30 @@ lemma override_out_in: "f \<oplus> (g \<oplus> h on (out a)) on (in b) = f \<opl
 lemma override_in_out: "f \<oplus> (g \<oplus> h on (in a)) on (out b) = f \<oplus> g on (out b)"
   by (metis Diff_triv in_out_disj inf_commute override_on_cancel4)
 
-lemma homalph_in[simp]: "in (homalph a) = in a \<union> undash ` out a"
-  apply(simp add:homalph_def)
-  apply (smt Un_commute Un_empty_left in_alphabet_def in_dash inf_absorb2 inf_commute le_infI1 order_refl out_alphabet_def undash_dashed)
-done
+lemma homalph_in[var]: "in (homalph a) = in a \<union> undash ` out a"
+  by (simp add:var homalph_def)
 
-lemma homalph_out[simp]: "out (homalph a) = out a \<union> dash ` in a"
-  apply (simp add:homalph_def)
-  apply(metis out_dash_in out_undash_out sup_bot_left)
-done
+lemma homalph_out[var]: "out (homalph a) = out a \<union> dash ` in a"
+  by (simp add:homalph_def var)
 
-lemma dash_dist_inter: "dash ` (x \<inter> y) = dash ` x \<inter> dash ` y"
-  by (metis image_Int inj_dash)
+lemma dash_dist_inter[var]: "dash ` (x \<inter> y) = dash ` x \<inter> dash ` y"
+  by (metis image_Int dash_inj)
 
-lemma dash_dist_union: "dash ` (x \<union> y) = dash ` x \<union> dash ` y"
+lemma dash_dist_union[var]: "dash ` (x \<union> y) = dash ` x \<union> dash ` y"
   by (metis image_Un)
 
-lemma homalph_homogeneous: "HOMOGENEOUS (homalph a)"
-  apply(simp add:HOMOGENEOUS_def)
-  apply (metis VAR.dash_undash_out image_Un sup_commute)
-done
+lemma homalph_homogeneous[var]: "HOMOGENEOUS (homalph a)"
+  by (auto simp add:HOMOGENEOUS_def var)
   
-lemma homogeneous_homalpha: "\<lbrakk> a \<subseteq> UNDASHED \<union> DASHED ; HOMOGENEOUS a \<rbrakk> \<Longrightarrow> homalph a = a"
-apply(simp add:HOMOGENEOUS_def homalph_def)
-  by (smt Int_Un_distrib Int_Un_distrib2 Un_absorb in_alphabet_def le_iff_inf out_alphabet_def undash_dash')
+lemma homogeneous_homalpha[var]: "\<lbrakk> a \<subseteq> UNDASHED \<union> DASHED ; HOMOGENEOUS a \<rbrakk> \<Longrightarrow> homalph a = a"
+  apply(simp add:HOMOGENEOUS_def homalph_def var)
+  apply(metis in_out_complete sup_idem undash_dash')
+done
 
-lemma homalpha_dashes[simp]: "homalph a \<subseteq> UNDASHED \<union> DASHED"
-  by (metis Un_mono homalph_in homalph_out in_undashed out_undashed homalph_def)
+lemma homalpha_dashes[var]: "homalph a \<subseteq> UNDASHED \<union> DASHED"
+  by (simp add:homalph_def var)
 
-lemma homalpha_subset[simp]: "a \<subseteq> UNDASHED \<union> DASHED \<Longrightarrow> a \<subseteq> homalph a"
+lemma homalpha_subset[var]: "a \<subseteq> UNDASHED \<union> DASHED \<Longrightarrow> a \<subseteq> homalph a"
 proof (simp add:homalph_def)
   assume "a \<subseteq> UNDASHED \<union> DASHED"
   moreover hence "a = in a \<union> out a"
@@ -296,42 +264,8 @@ proof (simp add:homalph_def)
 qed
 
 
-lemma homalpha_mono[simp]: "a \<subseteq> b \<Longrightarrow> homalph a \<subseteq> homalph b"
-  by (auto simp add:homalph_def utp_alphabet_simps)
-
-(*
-lemma homalph_minus: "homalph (a - b) = homalph a - (b - homalph a)"
-proof
-  show "homalph (a - b) \<subseteq> homalph a - (b - homalph a)"
-    by (metis Diff_disjoint Diff_subset Diff_triv homalpha_mono)
-next
-  show "homalph a - (b - homalph a) \<subseteq> homalph (a - b)"
-    apply(auto)
-    apply(simp add:homalph_def)
-    apply(auto)
-    apply (metis DiffI Int_iff in_alphabet_def)
-    apply(simp add:image_def undash_def dash_def utp_alphabet_simps)
-    apply(auto)
-    apply(force)
-    
-  apply(clarify)
-  apply(fast)
-
-
-lemma homalpha_in_minus: "b \<subseteq> out a \<Longrightarrow> in (homalph (a - b)) = in (homalph a)"
-proof
-  assume assm:"b \<subseteq> out a"
-  thus "in (homalph (a - b)) \<subseteq> in (homalph a)"
-    by (metis Diff_subset VAR.homalpha_mono in_alphabet_def inf_mono set_eq_subset)
-
-next
-  assume assm:"b \<subseteq> out a"
-  thus "in (homalph a) \<subseteq> in (homalph (a - b))"
-    
-  
- apply(simp add:homalph_def)
- apply(safe)
-*)
+lemma homalpha_mono[var]: "a \<subseteq> b \<Longrightarrow> homalph a \<subseteq> homalph b"
+  by (auto simp add:homalph_def utp_alphabet_simps var)
 
 end
 end
