theories/generic/utp_lattice.thy
@@ -71,14 +71,7 @@ subsection {* Theorems *}
 
 text {* Making the theorem below a default dest rule incurs problems?! *}
 
-theorem WF_ALPHA_PREDICATE_OVER_closure :
-"\<lbrakk>a \<in> WF_ALPHABET;
- p \<in> WF_ALPHA_PREDICATE_OVER a\<rbrakk> \<Longrightarrow>
- p \<in> WF_ALPHA_PREDICATE"
-apply (simp add: WF_ALPHA_PREDICATE_OVER_def)
-done
-
-theorem WF_BINDING_SET_Union [intro] :
+theorem WF_BINDING_SET_Union [intro,binding] :
 "ps \<subseteq> WF_BINDING_SET a \<Longrightarrow>
  \<Union> ps \<in> WF_BINDING_SET a"
 apply (simp add: Union_eq WF_BINDING_SET_def)
@@ -88,7 +81,7 @@ apply (rule_tac x = "x" in bexI)
 apply (auto)
 done
 
-theorem WF_BINDING_SET_Inter [intro] :
+theorem WF_BINDING_SET_Inter [intro,binding] :
 "\<lbrakk>ps \<subseteq> WF_BINDING_SET a; ps \<noteq> {}\<rbrakk> \<Longrightarrow>
  \<Inter> ps \<in> WF_BINDING_SET a"
 apply (simp add: WF_BINDING_SET_def)
@@ -97,51 +90,46 @@ done
 
 subsubsection {* Closure Theorems *}
 
-theorem BotP_closure [simp] :
+theorem BotP_closure [closure] :
 "a \<in> WF_ALPHABET \<Longrightarrow>
  (\<bottom>p a) \<in> WF_ALPHA_PREDICATE"
-apply (simp add: BotP_def)
-done
+  by (simp add: BotP_def closure)
 
-theorem TopP_closure [simp] :
+
+theorem TopP_closure [closure] :
 "a \<in> WF_ALPHABET \<Longrightarrow>
  (\<top>p a) \<in> WF_ALPHA_PREDICATE"
-apply (simp add: TopP_def)
-done
+  by (simp add: TopP_def closure)
 
-theorem SupP_closure [simp] :
+theorem SupP_closure [closure] :
 "\<lbrakk>a \<in> WF_ALPHABET;
  ps \<subseteq> WF_ALPHA_PREDICATE_OVER a\<rbrakk> \<Longrightarrow>
  \<Squnion> a ps \<in> WF_ALPHA_PREDICATE"
 apply (case_tac "ps = {}")
-apply (simp add: SupP_def)
-apply (simp add: SupP_def)
-apply (simp add: WF_ALPHA_PREDICATE_OVER_def WF_ALPHA_PREDICATE_def)
-apply (safe)
-apply (auto) [1]
-apply (rule WF_BINDING_SET_Inter)
-apply (auto)
-apply (subgoal_tac "\<Union> {\<alpha> p | p . p \<in> ps} = \<alpha> p")
-apply (auto)
+apply (simp add: SupP_def alphabet closure)+
+apply (subgoal_tac "\<Union> {\<alpha> p | p . p \<in> ps} = a")
+apply(auto simp add:WF_ALPHA_PREDICATE_def)[1]
+apply(simp add:WF_ALPHA_PREDICATE_OVER_def)
+apply(auto simp add:WF_ALPHA_PREDICATE_OVER_def WF_ALPHA_PREDICATE_def)[1]
+apply(subgoal_tac "{\<beta> p |p. p \<in> ps} \<subseteq> WF_BINDING_SET (\<Union>{\<alpha> p |p. p \<in> ps})")
+apply(auto simp add:WF_ALPHA_PREDICATE_OVER_def WF_ALPHA_PREDICATE_def)
 done
 
-theorem InfP_closure [simp] :
+theorem InfP_closure [closure] :
 "\<lbrakk>a \<in> WF_ALPHABET;
- ps \<subseteq> WF_ALPHA_PREDICATE_OVER a\<rbrakk> \<Longrightarrow>
+ps \<subseteq> WF_ALPHA_PREDICATE_OVER a\<rbrakk> \<Longrightarrow>
  \<Sqinter> a ps \<in> WF_ALPHA_PREDICATE"
 apply (case_tac "ps = {}")
-apply (simp add: InfP_def)
-apply (simp add: InfP_def)
-apply (simp add: WF_ALPHA_PREDICATE_OVER_def WF_ALPHA_PREDICATE_def)
-apply (safe)
-apply (auto) [1]
-apply (rule WF_BINDING_SET_Union)
-apply (auto)
-apply (subgoal_tac "\<Union> {\<alpha> p | p . p \<in> ps} = \<alpha> p")
-apply (auto)
+apply (simp add: InfP_def alphabet closure)+
+apply (subgoal_tac "\<Union> {\<alpha> p | p . p \<in> ps} = a")
+apply (auto simp add: WF_ALPHA_PREDICATE_def)[1]
+apply(simp add:WF_ALPHA_PREDICATE_OVER_def)
+apply(auto simp add:WF_ALPHA_PREDICATE_OVER_def WF_ALPHA_PREDICATE_def)[1]
+apply(subgoal_tac "{\<beta> p |p. p \<in> ps} \<subseteq> WF_BINDING_SET (\<Union>{\<alpha> p |p. p \<in> ps})")
+apply(auto simp add:WF_ALPHA_PREDICATE_OVER_def WF_ALPHA_PREDICATE_def)
 done
 
-theorem WFP_closure [simp] :
+theorem WFP_closure [closure] :
 "\<lbrakk>a \<in> WF_ALPHABET;
  f \<in> WF_ALPHA_FUNCTION_BETWEEN a a\<rbrakk> \<Longrightarrow>
  \<mu> a f \<in> WF_ALPHA_PREDICATE"
@@ -150,7 +138,7 @@ apply (rule SupP_closure)
 apply (auto)
 done
 
-theorem SFP_closure [simp] :
+theorem SFP_closure [closure] :
 "\<lbrakk>a \<in> WF_ALPHABET;
  f \<in> WF_ALPHA_FUNCTION_BETWEEN a a\<rbrakk> \<Longrightarrow>
  \<nu> a f \<in> WF_ALPHA_PREDICATE"
@@ -161,50 +149,50 @@ done
 
 subsubsection {* Alphabet Theorems *}
 
-theorem BotP_alphabet [simp] :
+theorem BotP_alphabet [alphabet] :
 "a \<in> WF_ALPHABET \<Longrightarrow>
  \<alpha> (\<bottom>p a) = a"
-apply (simp add: BotP_def)
+apply (simp add: BotP_def closure alphabet)
 done
 
-theorem TopP_alphabet [simp] :
+theorem TopP_alphabet [alphabet] :
 "a \<in> WF_ALPHABET \<Longrightarrow>
  \<alpha> (\<top>p a) = a"
-apply (simp add: TopP_def)
+apply (simp add: TopP_def closure alphabet)
 done
 
-theorem SupP_alphabet [simp] :
+theorem SupP_alphabet [alphabet] :
 "\<lbrakk>a \<in> WF_ALPHABET;
  ps \<subseteq> WF_ALPHA_PREDICATE_OVER a\<rbrakk> \<Longrightarrow>
  \<alpha> (\<Squnion> a ps) = a"
 apply (simp add: SupP_def WF_ALPHA_PREDICATE_OVER_def)
-apply (auto)
+apply (auto simp add:alphabet)
 done
 
-theorem InfP_alphabet [simp] :
+theorem InfP_alphabet [alphabet] :
 "\<lbrakk>a \<in> WF_ALPHABET;
  ps \<subseteq> WF_ALPHA_PREDICATE_OVER a\<rbrakk> \<Longrightarrow>
  \<alpha> (\<Sqinter> a ps) = a"
 apply (simp add: InfP_def WF_ALPHA_PREDICATE_OVER_def)
-apply (auto)
+apply (auto simp add:alphabet)
 done
 
-theorem WFP_alphabet [simp] :
+theorem WFP_alphabet [alphabet] :
 "\<lbrakk>a \<in> WF_ALPHABET;
  f \<in> WF_ALPHA_FUNCTION_BETWEEN a a\<rbrakk> \<Longrightarrow>
  \<alpha> (\<mu> a f) = a"
 apply (simp add: WFP_def)
 apply (subst SupP_alphabet)
-apply (auto)
+apply (auto simp add:alphabet)
 done
 
-theorem SFP_alphabet [simp] :
+theorem SFP_alphabet [alphabet] :
 "\<lbrakk>a \<in> WF_ALPHABET;
  f \<in> WF_ALPHA_FUNCTION_BETWEEN a a\<rbrakk> \<Longrightarrow>
  \<alpha> (\<nu> a f) = a"
 apply (simp add: SFP_def)
 apply (subst InfP_alphabet)
-apply (auto)
+apply (auto simp add:alphabet)
 done
 
 subsubsection {* Evaluation Theorems *}
@@ -217,7 +205,7 @@ theorem EvalP_InfP [eval] :
  ps \<subseteq> WF_ALPHA_PREDICATE_OVER a;
  b \<in> WF_BINDING\<rbrakk> \<Longrightarrow>
  EvalP (\<Sqinter> a ps) b = (\<exists> p \<in> ps . EvalP p b)"
-apply (simp add: EvalP_def)
+apply (simp add: EvalP_def closure)
 apply (simp add: InfP_def)
 apply (safe)
 -- {* Subgoal 1 *}
@@ -226,7 +214,7 @@ apply (simp add: TopP_def FalseP_def)
 apply (rule_tac x = "p" in bexI)
 apply (subgoal_tac "p \<in> WF_ALPHA_PREDICATE")
 apply (simp add: EvalP_def)
-apply (auto dest: WF_ALPHA_PREDICATE_OVER_closure) [1]
+apply (auto dest: WF_ALPHA_PREDICATE_OVER_dest) [1]
 apply (assumption)
 -- {* Subgoal 3 *}
 apply (rule_tac x = "\<beta> p" in exI)
@@ -235,7 +223,7 @@ apply (rule_tac x = "p" in exI)
 apply (simp)
 apply (subgoal_tac "p \<in> WF_ALPHA_PREDICATE")
 apply (simp add: EvalP_def)
-apply (auto dest: WF_ALPHA_PREDICATE_OVER_closure) [1]
+apply (auto dest: WF_ALPHA_PREDICATE_OVER_dest) [1]
 done
 
 theorem EvalP_SupP [eval] :
@@ -243,7 +231,7 @@ theorem EvalP_SupP [eval] :
  ps \<subseteq> WF_ALPHA_PREDICATE_OVER a;
  b \<in> WF_BINDING\<rbrakk> \<Longrightarrow>
  EvalP (\<Squnion> a ps) b = (\<forall> p \<in> ps . EvalP p b)"
-apply (simp add: EvalP_def)
+apply (simp add: EvalP_def closure)
 apply (simp add: SupP_def)
 apply (safe)
 -- {* Subgoal 1 *}
@@ -253,13 +241,13 @@ apply (drule_tac x = "\<beta> p" in spec)
 apply (subgoal_tac "p \<in> WF_ALPHA_PREDICATE")
 apply (simp add: EvalP_def)
 apply (auto) [1]
-apply (auto dest: WF_ALPHA_PREDICATE_OVER_closure) [1]
+apply (auto dest: WF_ALPHA_PREDICATE_OVER_dest) [1]
 -- {* Subgoal 3 *}
 apply (drule_tac x = "p" in bspec)
 apply (assumption)
 apply (subgoal_tac "p \<in> WF_ALPHA_PREDICATE")
 apply (simp add: EvalP_def)
-apply (auto dest: WF_ALPHA_PREDICATE_OVER_closure) [1]
+apply (auto dest: WF_ALPHA_PREDICATE_OVER_dest) [1]
 done
 
 declare WFP_def [eval]
@@ -277,157 +265,48 @@ abbreviation pred_order ::
 lemma SupP_lub :
   assumes "a \<in> WF_ALPHABET" "ps \<subseteq> WF_ALPHA_PREDICATE_OVER a"
   shows "least (pred_order a) (\<Squnion> a ps) (Upper (pred_order a) ps)"
-proof (auto simp add: least_def Upper_def)
-
-  from assms have r1: "ps \<subseteq> WF_ALPHA_PREDICATE"
-    by (auto simp add: WF_ALPHA_PREDICATE_OVER_def)
-
-  with assms have r2: "\<forall>x\<in>ps . \<alpha> (\<Squnion> a ps) = \<alpha> x"
-    by (auto simp add: SupP_def WF_ALPHA_PREDICATE_OVER_def)
-
-  with assms have r3: "\<forall>x\<in>ps . {\<beta> p | p . p \<in> ps} \<subseteq> WF_BINDING_SET (\<alpha> x)"
-    apply (auto simp only: WF_ALPHA_PREDICATE_OVER_def WF_ALPHA_PREDICATE_def)
-    apply (subgoal_tac "\<alpha> x = a")
-    apply (subgoal_tac "\<alpha> p = a")
-    apply (force)
-    apply (force)
-    apply (force)
-  done
-
-  with assms r1 have r4: "\<Squnion> a ps \<in> WF_ALPHA_PREDICATE"
-    by (simp add: SupP_closure)
-
-  fix x
-  show "\<lbrakk>x \<in> ps; x \<in> WF_ALPHA_PREDICATE_OVER a\<rbrakk> \<Longrightarrow> x \<sqsubseteq> \<Squnion> a ps"
-    proof -
-      assume assm1: "x \<in> ps" "x \<in> WF_ALPHA_PREDICATE_OVER a"
-      from assms assm1 r1 r2 r3 r4 show ?thesis
-        apply (simp add: SupP_def WF_ALPHA_PREDICATE_OVER_def)
-        apply (rule conjI)
-        apply (force)
-        apply (rule impI)
-        apply (utp_pred_taut_tac)
-        apply (auto simp add: EvalP_def)
-      done
-  qed
-
-  from assms r2 r4 show r6: "\<Squnion> a ps \<in> WF_ALPHA_PREDICATE_OVER a"
-    apply (simp add: WF_ALPHA_PREDICATE_OVER_def SupP_def)
-    apply (auto)
-  done
-
-  from assms r6 show
-    "\<lbrakk>x \<in> WF_ALPHA_PREDICATE_OVER a;
-     \<forall> y . y \<in> ps \<and> y \<in> WF_ALPHA_PREDICATE_OVER a \<longrightarrow> y \<sqsubseteq> x\<rbrakk> \<Longrightarrow> \<Squnion> a ps \<sqsubseteq> x"
-  proof -
-    assume assms': "x \<in> WF_ALPHA_PREDICATE_OVER a"
-      "\<forall> y . y \<in> ps \<and> y \<in> WF_ALPHA_PREDICATE_OVER a \<longrightarrow> y \<sqsubseteq> x"
-
-    with assms have r7: "\<alpha> (\<Squnion> a ps) = \<alpha> x"
-      by (simp add: WF_ALPHA_PREDICATE_OVER_def)
-
-    from assms assms' have r8: "x \<in> WF_ALPHA_PREDICATE"
-      by (simp add: WF_ALPHA_PREDICATE_OVER_def)
-
-    from assms assms' r4 r6 r7 r8 r1 show ?thesis
-    apply (simp add: WF_ALPHA_PREDICATE_OVER_def)
-    apply (auto)
-    apply (subgoal_tac "\<Squnion> (\<alpha> x) ps \<in> WF_ALPHA_PREDICATE")
-    apply (subgoal_tac "\<alpha> (\<Squnion> (\<alpha> x) ps) = \<alpha> x")
-    apply (utp_pred_taut_tac)
-    apply (simp add: EvalP_def)
-    apply (auto)
-    apply (subgoal_tac "\<alpha> x \<in> WF_ALPHABET")
-    apply (subgoal_tac "ps \<subseteq> WF_ALPHA_PREDICATE_OVER (\<alpha> x)")
-    apply (simp add: SupP_def)
-    apply (simp add: BotP_def)
-    apply (simp add: TrueP_def)
-    apply (force)
-    apply (simp add: WF_ALPHA_PREDICATE_OVER_def)
-    apply (force)
-    apply (metis (no_types) SupP_alphabet assms(1) assms(2) r7)
-    apply (metis (no_types) SupP_alphabet assms(1) assms(2) r7)
-    apply (metis (no_types) SupP_alphabet SupP_closure assms(1) assms(2) r7)
-  done
-qed
-qed
+  apply(insert assms)
+  apply(simp add:least_def Upper_def)
+  apply(auto intro!:eval_intro dest:WF_ALPHA_PREDICATE_OVER_dest intro:closure alpha_closure simp add:alphabet)
+  apply(simp add:eval closure alpha_closure WF_ALPHA_PREDICATE_OVER_def)
+  apply(simp add:eval closure alpha_closure WF_ALPHA_PREDICATE_OVER_def taut)
+  apply(auto)
+  apply(erule_tac x="p" in allE)
+  apply(auto)
+done
 
 lemma InfP_glb:
   assumes "a \<in> WF_ALPHABET" "ps \<subseteq> WF_ALPHA_PREDICATE_OVER a"
   shows "greatest (pred_order a) (\<Sqinter> a ps) (Lower (pred_order a) ps)"
-proof (auto simp add: greatest_def Lower_def)
-  fix x
-  assume assm1: "x \<in> ps" "x \<in> WF_ALPHA_PREDICATE_OVER a"
-  with assms show "\<Sqinter> a ps \<sqsubseteq> x"
-    apply (subgoal_tac "\<alpha> (\<Sqinter> a ps) = a")
-    apply (subgoal_tac "\<alpha> (\<Sqinter> a ps) = \<alpha> x")
-    apply (subgoal_tac "\<Sqinter> a ps \<in> WF_ALPHA_PREDICATE")
-    apply (simp add: InfP_def WF_ALPHA_PREDICATE_OVER_def)
-    apply (rule conjI)
-    apply (force)
-    apply (rule impI)
-    apply (utp_pred_taut_tac)
-    apply (simp add: EvalP_def)
-    apply (fast)
-    apply (simp add: InfP_closure)
-    apply (simp add: InfP_alphabet WF_ALPHA_PREDICATE_OVER_def)
-    apply (simp add: InfP_alphabet)
-  done
-  next
-
-  from assms show r1: "\<Sqinter> a ps \<in> WF_ALPHA_PREDICATE_OVER a"
-    by (simp add: WF_ALPHA_PREDICATE_OVER_def InfP_closure InfP_alphabet)
-
-  fix x
-  assume assm1: "x \<in> WF_ALPHA_PREDICATE_OVER a"
-    "\<forall> y . y \<in> ps \<and> y \<in> WF_ALPHA_PREDICATE_OVER a \<longrightarrow> x \<sqsubseteq> y"
-  with assms r1 show "x \<sqsubseteq> \<Sqinter> a ps"
-    apply (simp only: WF_ALPHA_PREDICATE_OVER_def)
-    apply (auto)
-    apply (utp_pred_taut_tac)
-    apply (simp add: EvalP_def)
-    apply (auto)
-    apply (subgoal_tac "\<alpha> x \<in> WF_ALPHABET")
-    apply (subgoal_tac "ps \<subseteq> WF_ALPHA_PREDICATE_OVER (\<alpha> x)")
-    apply (simp add: InfP_def)
-    apply (simp add: WF_ALPHA_PREDICATE_OVER_def)
-    apply (auto)
-    apply (case_tac "ps = {}")
-    apply (simp only: FalseP_def TopP_def)
-    apply (simp)
-    apply (simp only: FalseP_def TopP_def)
-    apply (simp)
-    apply (erule exE)
-    apply (erule conjE)
-    apply (erule exE)
-    apply (erule conjE)
-    apply (simp)
-    apply (erule_tac x = "p" in allE)
-    apply (force)
-    apply (simp add: WF_ALPHA_PREDICATE_OVER_def)
-    apply (force)
-  done
-qed
+  apply(insert assms)
+  apply(simp add:greatest_def Lower_def)
+  apply(auto intro!:eval_intro dest:WF_ALPHA_PREDICATE_OVER_dest intro:closure alpha_closure simp add:alphabet)
+  apply(simp add:eval closure alpha_closure WF_ALPHA_PREDICATE_OVER_def)
+  apply(force)
+  apply(simp add:eval closure alpha_closure WF_ALPHA_PREDICATE_OVER_def taut)
+  apply(auto)
+  apply(erule_tac x="p" in allE)
+  apply(auto)
+done
 
 lemma pred_complete_lattice [simp, intro!] :
   "a \<in> WF_ALPHABET \<Longrightarrow> complete_lattice (pred_order a)"
 apply (unfold_locales)
 apply (simp_all add: WF_ALPHA_PREDICATE_OVER_def)
 apply (auto)
-apply (utp_pred_taut_tac)
-apply (utp_pred_taut_tac)
-apply (rule_tac ballI)
-apply (erule_tac x = "b" in ballE)+
-apply (auto)
-apply (utp_pred_taut_tac)
+apply (simp add:eval taut closure alphabet alpha_closure)
+apply (simp add:eval taut closure alphabet alpha_closure)
+apply(force)
+apply (simp add:eval taut closure alphabet alpha_closure)
+apply (simp add:eval taut closure alphabet alpha_closure)
 apply (rule_tac x = "x \<and>p y" in exI)
 apply (simp add: least_def Upper_def)
 apply (safe)
-apply (utp_pred_taut_tac)+
+apply (simp add:eval taut closure alphabet alpha_closure)+
 apply (rule_tac x = "x \<or>p y" in exI)
 apply (simp add: greatest_def Lower_def)
 apply (safe)
-apply (utp_pred_taut_tac)+
+apply (simp add:eval taut closure alphabet alpha_closure)+
 apply (rule_tac x = "\<Squnion> a A" in exI)
 apply (insert SupP_lub)
 apply (auto simp add: WF_ALPHA_PREDICATE_OVER_def)
@@ -446,13 +325,13 @@ theorem InfP_Ref :
   shows "(\<Sqinter> a ps) \<sqsubseteq> p"
 proof -
   from assms have r1: "p \<in> WF_ALPHA_PREDICATE"
-    by (auto dest: WF_ALPHA_PREDICATE_OVER_closure)
+    by (auto dest: WF_ALPHA_PREDICATE_OVER_dest)
 
   from assms have r2: "\<alpha> p = a"
     by (auto simp: WF_ALPHA_PREDICATE_OVER_def)
 
   with assms r1 r2 show "(\<Sqinter> a ps) \<sqsubseteq> p"
-    by (utp_pred_taut_tac, auto)
+    by (auto simp add:eval taut closure alphabet alpha_closure)
 qed
 
 theorem SupP_Ref :
@@ -463,13 +342,13 @@ theorem SupP_Ref :
   shows "p \<sqsubseteq> (\<Squnion> a ps)"
 proof -
   from assms have r1: "p \<in> WF_ALPHA_PREDICATE"
-    by (auto dest: WF_ALPHA_PREDICATE_OVER_closure)
+    by (auto dest: WF_ALPHA_PREDICATE_OVER_dest)
 
   from assms have r2: "\<alpha> p = a"
     by (auto simp: WF_ALPHA_PREDICATE_OVER_def)
 
   with assms r1 r2 show "p \<sqsubseteq> (\<Squnion> a ps)"
-    by (utp_pred_taut_tac)
+    by (auto simp add:eval taut closure alphabet alpha_closure)
 qed
 end
 end
